Antimirov.v
@@ -1,0 +1,549 @@
+Require Import Coq.Program.Equality.
+Require Import Coq.Lists.List.
+
+Require Import KA.Utilities.
+Require Import KA.Finite.
+Require Import KA.Booleans.
+Require Import KA.Terms.
+Require Import KA.Scope.
+Local Open Scope ka_scope.
+
+Section AntimirovTypes.
+  Variable (A: Type).
+  Notation term := (term A).
+
+  Inductive derivative: term -> Type :=
+  | TOneOne:
+      derivative 1
+  | TLetterLetter:
+      forall (a: A),
+      derivative ($ a)
+  | TLetterOne:
+      forall {a: A},
+      derivative ($ a)
+  | TPlusLeft:
+      forall {t1: term} (t2: term),
+      derivative t1 ->
+      derivative (t1 + t2)
+  | TPlusRight:
+      forall (t1: term) {t2: term},
+      derivative t2 ->
+      derivative (t1 + t2)
+  | TTimesPre:
+      forall {t1: term} (t2: term),
+      derivative t1 ->
+      derivative (t1 ;; t2)
+  | TTimesPost:
+      forall (t1: term) {t2: term},
+      derivative t2 ->
+      derivative (t1 ;; t2)
+  | TStarInner:
+      forall (t: term),
+      derivative t ->
+      derivative (t *)
+  | TStarOne:
+      forall (t: term),
+      derivative (t *)
+  .
+
+  Inductive initial:
+    forall {t: term},
+    derivative t ->
+    Prop
+  :=
+  | InitialOneOne:
+      initial TOneOne
+  | InitialLetterLetter:
+      forall (a: A),
+      initial (TLetterLetter a)
+  | InitialPlusLeft:
+      forall (t1 t2: term) (d1: derivative t1),
+      initial d1 ->
+      initial (TPlusLeft t2 d1)
+  | InitialPlusRight:
+      forall (t1 t2: term) (d2: derivative t2),
+      initial d2 ->
+      initial (TPlusRight t1 d2)
+  | InitialTimesPre:
+      forall (t1 t2: term) (d1: derivative t1),
+      initial d1 ->
+      initial (TTimesPre t2 d1)
+  | InitialStarStep:
+      forall (t: term) (d: derivative t),
+      initial d ->
+      initial (TStarInner t d)
+  | InitialStarOne:
+      forall (t: term),
+      initial (TStarOne t)
+  .
+
+  Inductive nullable:
+    forall {t: term},
+    derivative t ->
+    Prop
+  :=
+  | NullableOneOne:
+      nullable TOneOne
+  | NullableLetterOne:
+      forall (a: A),
+      nullable (TLetterOne (a := a))
+  | NullablePlusLeft:
+      forall (t1 t2: term) (d: derivative t1),
+      nullable d ->
+      nullable (TPlusLeft t2 d)
+  | NullablePlusRight:
+      forall (t1 t2: term) (d: derivative t2),
+      nullable d ->
+      nullable (TPlusRight t1 d)
+  | NullableTimesPre:
+      forall (t1 t2: term) (d1: derivative t1) (d2: derivative t2),
+      nullable d1 ->
+      nullable d2 ->
+      initial d2 ->
+      nullable (TTimesPre t2 d1)
+  | NullableTimesPost:
+      forall (t1 t2: term) (d2: derivative t2),
+      nullable d2 ->
+      nullable (TTimesPost t1 d2)
+  | NullableStarInner:
+      forall (t: term) (d: derivative t),
+      nullable d ->
+      nullable (TStarInner t d)
+  | NullableStarOne:
+      forall (t: term),
+      nullable (TStarOne t)
+  .
+
+  Equations derivative_write {t: term} (d: derivative t): term := {
+    derivative_write TOneOne := 1;
+    derivative_write (TLetterLetter a) := $ a;
+    derivative_write TLetterOne := 1;
+    derivative_write (TPlusLeft _ d) := derivative_write d;
+    derivative_write (TPlusRight _ d) := derivative_write d;
+    derivative_write (TTimesPre t2 d) := derivative_write d ;; t2;
+    derivative_write (TTimesPost _ d) := derivative_write d;
+    derivative_write (TStarInner t d) := derivative_write d ;; t *;
+    derivative_write (TStarOne t) := 1;
+  }.
+End AntimirovTypes.
+
+Arguments TOneOne {A}.
+Arguments TLetterLetter {A}.
+Arguments TLetterOne {A} {a}.
+Arguments TPlusLeft {A} {t1} t2.
+Arguments TPlusRight {A} t1 {t2}.
+Arguments TTimesPre {A} {t1} t2.
+Arguments TTimesPost {A} t1 {t2}.
+Arguments TStarInner {A}.
+Arguments TStarOne {A}.
+Arguments derivative_write {A} {t}.
+
+Section AntimirovInitial.
+  Context {A: Type}.
+  Notation term := (term A).
+  Notation derivative := (derivative A).
+  Notation initial := (initial A).
+
+  Equations initial_b {t: term} (d: derivative t): bool := {
+    @initial_b 1 TOneOne := true;
+    @initial_b ($ a) (TLetterLetter a) := true;
+    @initial_b (t1 + t2) (TPlusLeft _ d1) := initial_b d1;
+    @initial_b (t1 + t2) (TPlusRight _ d2) := initial_b d2;
+    @initial_b (t1 ;; t2) (TTimesPre _ d1) := initial_b d1;
+    @initial_b (t*) (TStarInner _ d) := initial_b d;
+    @initial_b (t*) (TStarOne _) := true;
+    @initial_b _ _ := false;
+  }.
+
+  Lemma initial_dec (t: term) (d: derivative t):
+    initial d <-> initial_b d = true
+  .
+  Proof.
+    dependent induction d;
+    autorewrite with initial_b;
+    match goal with
+    | |- _ <-> true = true =>
+      split; intros; [reflexivity | constructor]
+    | |- _ <-> false = true =>
+      split; intros; [inversion H | discriminate]
+    | |- _ <-> initial_b d = true =>
+      split; intros; [
+        dependent destruction H |
+        constructor ];
+      intuition
+    end.
+  Qed.
+
+  Equations initial_l (t: term): list (derivative t) := {
+    initial_l 0 := nil;
+    initial_l 1 := TOneOne :: nil;
+    initial_l ($ a) := TLetterLetter a :: nil;
+    initial_l (t1 + t2) :=
+      map (TPlusLeft _) (initial_l t1) ++
+      map (TPlusRight _) (initial_l t2);
+    initial_l (t1 ;; t2) := map (TTimesPre t2) (initial_l t1);
+    initial_l (t*) := TStarOne t :: map (TStarInner t) (initial_l t);
+  }.
+
+  Lemma initial_list (t: term) (d: derivative t):
+    initial d <-> In d (initial_l t)
+  .
+  Proof.
+    dependent induction d;
+    autorewrite with initial_l;
+    autorewrite with initial_b;
+    try (split; intros; [now left | constructor]);
+    try (split; intros; [inversion H | now destruct H]).
+    - rewrite in_app_iff; repeat rewrite in_map_iff.
+      split; intros.
+      + dependent destruction H.
+        left; eexists.
+        intuition.
+      + constructor.
+        destruct H as [[d' [? ?]] | [d' [? ?]]].
+        * apply IHd.
+          inversion H.
+          now clean_exists.
+        * discriminate.
+    - rewrite in_app_iff; repeat rewrite in_map_iff.
+      split; intros.
+      + dependent destruction H.
+        right; eexists.
+        intuition.
+      + constructor.
+        destruct H as [[d' [? ?]] | [d' [? ?]]].
+        * discriminate.
+        * apply IHd.
+          inversion H.
+          now clean_exists.
+    - rewrite in_map_iff.
+      split; intros.
+      + dependent destruction H.
+        eexists.
+        intuition.
+      + constructor.
+        apply IHd.
+        destruct H as [d' [? ?]].
+        inversion H.
+        now clean_exists.
+    - rewrite in_map_iff.
+      split; intros.
+      + dependent destruction H.
+      + now destruct H as [d' [? ?]].
+    - simpl.
+      rewrite in_map_iff.
+      split; intros.
+      + dependent destruction H.
+        right.
+        eexists.
+        intuition.
+      + destruct H as [? | [d' [? ?]]];
+        try discriminate.
+        inversion H.
+        constructor.
+        clean_exists.
+        intuition.
+  Qed.
+
+  Lemma initial_reconstruct (t: term):
+    t == sum (map derivative_write (initial_l t))
+  .
+  Proof.
+    induction t.
+    - now vm_compute.
+    - vm_compute.
+      now rewrite EPlusUnit.
+    - vm_compute.
+      now rewrite EPlusUnit.
+    - autorewrite with initial_l.
+      rewrite map_app.
+      rewrite sum_split.
+      repeat rewrite map_map.
+      rewrite map_ext
+        with (f := (fun x => derivative_write (TPlusLeft t2 x)))
+             (g := derivative_write)
+        by easy.
+      rewrite map_ext
+        with (f := (fun x => derivative_write (TPlusRight t1 x)))
+             (g := derivative_write)
+        by easy.
+      now rewrite <- IHt1, <- IHt2.
+    - autorewrite with initial_l.
+      rewrite map_map.
+      rewrite map_ext with (g := (fun x => derivative_write x ;; t2)) by easy.
+      rewrite <- map_map with (g := fun x => x ;; t2).
+      rewrite sum_distribute_right.
+      now rewrite <- IHt1.
+    - autorewrite with initial_l.
+      simpl; autorewrite with sum.
+      autorewrite with derivative_write.
+      rewrite map_map.
+      rewrite map_ext with (g := (fun x => derivative_write x ;; t*)) by easy.
+      rewrite <- map_map with (g := fun x => x ;; t*).
+      rewrite sum_distribute_right.
+      rewrite <- IHt.
+      rewrite EStarLeft at 1.
+      now rewrite EPlusComm.
+  Qed.
+End AntimirovInitial.
+
+Section AntimirovNullable.
+  Context {A: Type}.
+  Notation term := (term A).
+  Notation derivative := (derivative A).
+  Notation nullable := (nullable A).
+
+  Equations nullable_b {t: term} (d: derivative t) : bool := {
+    @nullable_b 1 TOneOne := true;
+    @nullable_b ($ _) TLetterOne := true;
+    @nullable_b (t1 + t2) (TPlusLeft _ d) := nullable_b d;
+    @nullable_b (t1 + t2) (TPlusRight _ d) := nullable_b d;
+    @nullable_b (t1 ;; t2) (TTimesPre _ d) :=
+      nullable_b d && disj (map nullable_b (initial_l t2));
+    @nullable_b (t1 ;; t2) (TTimesPost _ d) :=
+      nullable_b d;
+    @nullable_b (t*) (TStarInner _ d) :=
+      nullable_b d;
+    @nullable_b (t*) (TStarOne _) := true;
+    @nullable_b _ _ := false;
+  }.
+
+  Lemma nullable_dec (t: term) (d: derivative t):
+    nullable d <-> nullable_b d = true
+  .
+  Proof.
+    dependent induction t;
+    dependent destruction d;
+    autorewrite with nullable_b;
+    match goal with
+    | |- _ <-> true = true =>
+      split; intros; [reflexivity | constructor]
+    | |- _ <-> false = true =>
+      split; intros; [inversion H | discriminate]
+    | |- _ <-> nullable_b _ = true =>
+      split; intros; [
+        dependent destruction H; intuition |
+        constructor ];
+      intuition
+    | _ => idtac
+    end.
+    split; intros.
+    - dependent destruction H.
+      apply andb_true_intro; split.
+      + now apply IHt1.
+      + apply disj_true.
+        apply in_map_iff.
+        exists d2.
+        split.
+        * now apply IHt2.
+        * now apply initial_list.
+    - apply andb_prop in H; destruct H.
+      apply disj_true in H0.
+      apply in_map_iff in H0.
+      destruct H0 as [d' [? ?]].
+      eapply NullableTimesPre.
+      + now apply IHt1.
+      + apply IHt2.
+        apply H0.
+      + now apply initial_list.
+  Qed.
+End AntimirovNullable.
+
+Section AntimirovDerive.
+  Context {A: Type}.
+  Context `{Finite A}.
+  Notation term := (term A).
+  Notation derivative := (derivative A).
+  Notation initial := (initial A).
+  Notation nullable := (nullable A).
+
+  Inductive derive (a: A):
+    forall {t: term},
+    derivative t ->
+    derivative t ->
+    Prop
+  :=
+  | DeriveLetterLetter: derive a (TLetterLetter a) TLetterOne
+  | DerivePlusLeft:
+      forall (t1 t2: term) (d11 d12: derivative t1),
+      derive a d11 d12 ->
+      derive a (TPlusLeft t2 d11) (TPlusLeft t2 d12)
+  | DerivePlusRight:
+      forall (t1 t2: term) (d21 d22: derivative t2),
+      derive a d21 d22 ->
+      derive a (TPlusRight t1 d21) (TPlusRight t1 d22)
+  | DeriveTimesPre:
+      forall (t1 t2: term) (d11 d12: derivative t1),
+      derive a d11 d12 ->
+      derive a (TTimesPre t2 d11) (TTimesPre t2 d12)
+  | DeriveTimesJump:
+      forall (t1 t2: term) (d1: derivative t1) (i d2: derivative t2),
+      nullable d1 ->
+      initial i ->
+      derive a i d2 ->
+      derive a (TTimesPre t2 d1) (TTimesPost t1 d2)
+  | DeriveTimesPost:
+      forall (t1 t2: term) (d21 d22: derivative t2),
+      derive a d21 d22 ->
+      derive a (TTimesPost t1 d21) (TTimesPost t1 d22)
+  | DeriveStarInnerStep:
+      forall (t: term) (d1 d2: derivative t),
+      derive a d1 d2 ->
+      derive a (TStarInner t d1) (TStarInner t d2)
+  | DeriveStarInnerJump:
+      forall (t: term) (d1 i d2: derivative t),
+      nullable d1 ->
+      initial i ->
+      derive a i d2 ->
+      derive a (TStarInner t d1) (TStarInner t d2)
+  .
+
+  Equations derive_b (a: A) {t: term} (d1 d2: derivative t): bool := {
+    derive_b a (TLetterLetter a') TLetterOne :=
+      if finite_dec a a' then true else false;
+    derive_b a (TPlusLeft _ d1) (TPlusLeft _ d2) := derive_b a d1 d2;
+    derive_b a (TPlusRight _ d1) (TPlusRight _ d2) := derive_b a d1 d2;
+    derive_b a (TTimesPre _ d1) (TTimesPre _ d2) := derive_b a d1 d2;
+    derive_b a (TTimesPre t2 d1) (TTimesPost _ d2) :=
+      nullable_b d1 && disj (map (fun i => derive_b a i d2) (initial_l t2));
+    derive_b a (TTimesPost _ d1) (TTimesPost _ d2) := derive_b a d1 d2;
+    derive_b a (TStarInner _ d1) (TStarInner _ d2) :=
+      derive_b a d1 d2 || (
+        nullable_b d1 &&
+        disj (map (fun i => derive_b a i d2) (initial_l t))
+      );
+    derive_b _ _ _ := false;
+  }.
+
+  Lemma derive_dec (t: term) (d1 d2: derivative t) (a: A):
+    derive a d1 d2 <-> derive_b a d1 d2 = true
+  .
+  Proof.
+    dependent induction t;
+    dependent destruction d1;
+    dependent destruction d2;
+    autorewrite with derive_b;
+    match goal with
+    | |- _ <-> true = true =>
+      split; intros; [reflexivity | constructor]
+    | |- _ <-> false = true =>
+      split; intros; [now inversion H0 | discriminate]
+    | |- _ <-> derive_b _ _ _ = true =>
+      split; intros; [
+        dependent destruction H0; intuition |
+        constructor ];
+      intuition
+    | _ => idtac
+    end.
+    - destruct (finite_dec a0 a); split; intros.
+      + reflexivity.
+      + subst; constructor.
+      + now inversion H0.
+      + discriminate.
+    - split; intros.
+      + dependent destruction H0.
+        apply andb_true_intro; split.
+        * now apply nullable_dec.
+        * apply disj_true.
+          apply in_map_iff.
+          eexists.
+          intuition.
+          now apply initial_list.
+      + apply andb_prop in H0; destruct H0.
+        apply disj_true in H1.
+        apply in_map_iff in H1.
+        destruct H1 as [i [? ?]].
+        eapply DeriveTimesJump.
+        * now apply nullable_dec.
+        * apply initial_list, H2.
+        * now apply IHt2.
+    - split; intros.
+      + apply Bool.orb_true_intro.
+        dependent destruction H0.
+        * left.
+          now apply IHt.
+        * right.
+          apply andb_true_intro; split.
+          -- now apply nullable_dec.
+          -- apply disj_true.
+             apply in_map_iff.
+             exists i.
+             intuition.
+             now apply initial_list.
+      + apply Bool.orb_true_elim in H0.
+        destruct H0.
+        * apply DeriveStarInnerStep.
+          now apply IHt.
+        * apply andb_prop in e; destruct e.
+          apply disj_true in H1.
+          apply in_map_iff in H1.
+          destruct H1 as [i [? ?]].
+          eapply DeriveStarInnerJump.
+          -- now apply nullable_dec.
+          -- apply initial_list, H2.
+          -- now apply IHt.
+  Qed.
+
+  Equations derive_list (t: term) : list (derivative t) := {
+    derive_list 0 := nil;
+    derive_list 1 := TOneOne :: nil;
+    derive_list ($ a) := TLetterLetter a :: TLetterOne :: nil;
+    derive_list (t1 + t2) :=
+      map (TPlusLeft _) (derive_list t1) ++
+      map (TPlusRight _) (derive_list t2);
+    derive_list (t1 ;; t2) :=
+      map (TTimesPre _) (derive_list t1) ++
+      map (TTimesPost _) (derive_list t2);
+    derive_list (t*) :=
+      TStarOne _ :: map (TStarInner _) (derive_list t);
+  }.
+
+  Equations derive_eqb {t: term} (d1 d2: derivative t) : bool := {
+    derive_eqb TOneOne TOneOne := true;
+    derive_eqb (TLetterLetter _) (TLetterLetter _) := true;
+    derive_eqb TLetterOne TLetterOne := true;
+    derive_eqb (TPlusLeft _ d1) (TPlusLeft _ d2) := derive_eqb d1 d2;
+    derive_eqb (TPlusRight _ d1) (TPlusRight _ d2) := derive_eqb d1 d2;
+    derive_eqb (TTimesPre _ d1) (TTimesPre _ d2) := derive_eqb d1 d2;
+    derive_eqb (TTimesPost _ d1) (TTimesPost _ d2) := derive_eqb d1 d2;
+    derive_eqb (TStarOne _) (TStarOne _) := true;
+    derive_eqb (TStarInner _ d1) (TStarInner _ d2) := derive_eqb d1 d2;
+    derive_eqb _ _ := false;
+  }.
+
+  Lemma derive_eqb_correct (t: term) (d1 d2: derivative t):
+    derive_eqb d1 d2 = true <-> d1 = d2
+  .
+  Proof.
+    dependent induction t;
+    dependent destruction d1;
+    dependent destruction d2;
+    autorewrite with derive_eqb;
+    try easy.
+    - rewrite IHt1.
+      split; intros.
+      + now subst.
+      + apply Eqdep.EqdepTheory.inj_pair2.
+        now inversion H0.
+    - rewrite IHt2.
+      split; intros.
+      + now subst.
+      + apply Eqdep.EqdepTheory.inj_pair2.
+        now inversion H0.
+    - rewrite IHt1.
+      split; intros.
+      + now subst.
+      + apply Eqdep.EqdepTheory.inj_pair2.
+        now inversion H0.
+    - rewrite IHt2.
+      split; intros.
+      + now subst.
+      + apply Eqdep.EqdepTheory.inj_pair2.
+        now inversion H0.
+    - rewrite IHt.
+      split; intros.
+      + now subst.
+      + apply Eqdep.EqdepTheory.inj_pair2.
+        now inversion H0.
+  Qed.
+End AntimirovDerive.
