Booleans.v
@@ -1,0 +1,31 @@
+From Equations Require Import Equations.
+Require Import Coq.Lists.List.
+
+Equations conj (l: list bool) : bool := {
+  conj nil := true;
+  conj (b :: l) := b && (conj l);
+}.
+
+Equations disj (l: list bool) : bool := {
+  disj nil := false;
+  disj (b :: l) := b || (disj l);
+}.
+
+Lemma disj_true (l: list bool):
+  disj l = true <-> In true l
+.
+Proof.
+  split; intros.
+  - induction l; autorewrite with disj in H.
+    + discriminate.
+    + destruct a.
+      * now left.
+      * right.
+        intuition.
+  - induction l.
+    + contradiction.
+    + destruct a; simpl.
+      * now autorewrite with disj.
+      * apply IHl.
+        now destruct H.
+Qed.
