Utilities.v
@@ -1,0 +1,8 @@
+Require Coq.Program.Equality.
+
+Ltac clean_exists :=
+  repeat match goal with
+  | H: existT ?P ?p _ = existT ?P ?p _ |- _ =>
+    apply Eqdep.EqdepTheory.inj_pair2 in H
+         end;
+  subst.
